proof/ConRon/Generated/FunsExternal_Template.lean
@@ -60,33 +60,33 @@ axiom alloc.sync.Arc.Insts.CoreOpsDerefDeref.deref
   {T : Type} (A : Type) : alloc.sync.Arc T → Result T
 
 /-- [con_ron_core::ron::node::dup]:
-    Source: 'crates/con-ron-core/src/ron/node.rs', lines 484:0-491:1
+    Source: 'crates/con-ron-core/src/ron/node.rs', lines 301:0-303:1
     Visibility: public -/
 axiom ron.node.dup : kernel.expr.Expr → Result kernel.expr.Expr
 
 /-- [con_ron_core::ron::node::view]:
-    Source: 'crates/con-ron-core/src/ron/node.rs', lines 319:0-367:1
+    Source: 'crates/con-ron-core/src/ron/node.rs', lines 209:0-222:1
     Visibility: public -/
 axiom ron.node.view : kernel.expr.Expr → Result ron.node.ExprView
 
 /-- [con_ron_core::ron::node::{impl core::ops::drop::Drop for con_ron_core::kernel::expr::Expr}::drop]:
-    Source: 'crates/con-ron-core/src/ron/node.rs', lines 566:4-568:5
+    Source: 'crates/con-ron-core/src/ron/node.rs', lines 319:4-321:5
     Visibility: public -/
 axiom kernel.expr.Expr.Insts.CoreOpsDropDrop.drop
   : kernel.expr.Expr → Result kernel.expr.Expr
 
 /-- [con_ron_core::ron::node::ptr_eq]:
-    Source: 'crates/con-ron-core/src/ron/node.rs', lines 500:0-502:1
+    Source: 'crates/con-ron-core/src/ron/node.rs', lines 308:0-310:1
     Visibility: public -/
 axiom ron.node.ptr_eq : kernel.expr.Expr → kernel.expr.Expr → Result Bool
 
 /-- [con_ron_core::ron::node::data]:
-    Source: 'crates/con-ron-core/src/ron/node.rs', lines 477:0-479:1
+    Source: 'crates/con-ron-core/src/ron/node.rs', lines 295:0-297:1
     Visibility: public -/
 axiom ron.node.data : kernel.expr.Expr → Result Std.U64
 
 /-- [con_ron_core::ron::node::alloc_proj]:
-    Source: 'crates/con-ron-core/src/ron/node.rs', lines 465:0-467:1
+    Source: 'crates/con-ron-core/src/ron/node.rs', lines 284:0-286:1
     Visibility: public -/
 axiom ron.node.alloc_proj
   :
@@ -94,7 +94,7 @@ axiom ron.node.alloc_proj
     kernel.expr.Expr
 
 /-- [con_ron_core::ron::node::alloc_let_e]:
-    Source: 'crates/con-ron-core/src/ron/node.rs', lines 451:0-453:1
+    Source: 'crates/con-ron-core/src/ron/node.rs', lines 272:0-274:1
     Visibility: public -/
 axiom ron.node.alloc_let_e
   :
@@ -102,7 +102,7 @@ axiom ron.node.alloc_let_e
     Result kernel.expr.Expr
 
 /-- [con_ron_core::ron::node::alloc_forall_e]:
-    Source: 'crates/con-ron-core/src/ron/node.rs', lines 444:0-446:1
+    Source: 'crates/con-ron-core/src/ron/node.rs', lines 266:0-268:1
     Visibility: public -/
 axiom ron.node.alloc_forall_e
   :
@@ -110,7 +110,7 @@ axiom ron.node.alloc_forall_e
     → Result kernel.expr.Expr
 
 /-- [con_ron_core::ron::node::alloc_lam]:
-    Source: 'crates/con-ron-core/src/ron/node.rs', lines 437:0-439:1
+    Source: 'crates/con-ron-core/src/ron/node.rs', lines 260:0-262:1
     Visibility: public -/
 axiom ron.node.alloc_lam
   :
@@ -118,14 +118,14 @@ axiom ron.node.alloc_lam
     → Result kernel.expr.Expr
 
 /-- [con_ron_core::ron::node::alloc_app]:
-    Source: 'crates/con-ron-core/src/ron/node.rs', lines 430:0-432:1
+    Source: 'crates/con-ron-core/src/ron/node.rs', lines 254:0-256:1
     Visibility: public -/
 axiom ron.node.alloc_app
   :
   Std.U64 → kernel.expr.Expr → kernel.expr.Expr → Result kernel.expr.Expr
 
 /-- [con_ron_core::ron::node::alloc_const]:
-    Source: 'crates/con-ron-core/src/ron/node.rs', lines 423:0-425:1
+    Source: 'crates/con-ron-core/src/ron/node.rs', lines 248:0-250:1
     Visibility: public -/
 axiom ron.node.alloc_const
   :
@@ -133,24 +133,24 @@ axiom ron.node.alloc_const
     kernel.level.Level) → Result kernel.expr.Expr
 
 /-- [con_ron_core::ron::node::alloc_sort]:
-    Source: 'crates/con-ron-core/src/ron/node.rs', lines 416:0-418:1
+    Source: 'crates/con-ron-core/src/ron/node.rs', lines 242:0-244:1
     Visibility: public -/
 axiom ron.node.alloc_sort
   : Std.U64 → kernel.level.Level → Result kernel.expr.Expr
 
 /-- [con_ron_core::ron::node::alloc_fvar]:
-    Source: 'crates/con-ron-core/src/ron/node.rs', lines 409:0-411:1
+    Source: 'crates/con-ron-core/src/ron/node.rs', lines 236:0-238:1
     Visibility: public -/
 axiom ron.node.alloc_fvar
   : Std.U64 → Std.U64 → kernel.expr.Expr → Result kernel.expr.Expr
 
 /-- [con_ron_core::ron::node::alloc_bvar]:
-    Source: 'crates/con-ron-core/src/ron/node.rs', lines 402:0-404:1
+    Source: 'crates/con-ron-core/src/ron/node.rs', lines 230:0-232:1
     Visibility: public -/
 axiom ron.node.alloc_bvar : Std.U64 → Std.U64 → Result kernel.expr.Expr
 
 /-- [con_ron_core::ron::node::alloc_lit]:
-    Source: 'crates/con-ron-core/src/ron/node.rs', lines 458:0-460:1
+    Source: 'crates/con-ron-core/src/ron/node.rs', lines 278:0-280:1
     Visibility: public -/
 axiom ron.node.alloc_lit
   : Std.U64 → kernel.expr.Literal → Result kernel.expr.Expr
